src/lib/state/DY.Lib.State.Tagged.fst
@@ -45,14 +45,12 @@ let split_local_bytes_state_predicate_func {|crypto_invariants|} : split_functio
 
   tag_set_t = string;
   tag_t = string;
-  is_disjoint = default_disjoint;
+  is_disjoint = unequal;
   tag_belong_to = (fun dtag tag -> dtag = tag);
   cant_belong_to_disjoint_sets = (fun dtag tag1 tag2 -> ());
 
   raw_data_t = trace & principal & state_id & bytes;
   output_t = prop;
-
-  default_global_fun = (fun tr prin sess_id sess_content -> False);
 
   decode_tagged_data = (fun (tr, prin, sess_id, sess_content) -> (
     match parse tagged_state sess_content with
@@ -60,8 +58,10 @@ let split_local_bytes_state_predicate_func {|crypto_invariants|} : split_functio
     | None -> None
   ));
 
-  local_fun = local_bytes_state_predicate;
-  global_fun = trace -> principal -> state_id -> bytes -> prop;
+  local_fun_t = local_bytes_state_predicate;
+  global_fun_t = trace -> principal -> state_id -> bytes -> prop;
+
+  default_global_fun = (fun tr prin sess_id sess_content -> False);
 
   apply_local_fun = (fun spred (tr, prin, sess_id, content) ->
     spred.pred tr prin sess_id content
